src/class/FStarC.Class.Ord.fsti
@@ -31,7 +31,7 @@ val sort_dedup
 (* Returns the difference of two lists, modulo order and duplication.
 The first component is the elements only present in xs, and the second
 is the elements only present in ys. *)
-val ord_list_diff (#a:Type) {| ord a |} (xs ys : list a) : list a & list a
+val ord_list_diff (#a:Type0) {| ord a |} (xs ys : list a) : list a & list a
 
 instance val ord_eq (a:Type) (d : ord a) : Tot (deq a)
 
